Examples/PrintCalc.thy
@@ -1,0 +1,111 @@
+theory PrintCalc imports
+ "../MergeableTc/Mergeable" "../MergeableTc/MergeableInstances" "../MergeableTc/SplittableInstances" HOL.Lifting HOL.Lifting_Set "../MergeSemTc/LiftUtils"
+begin
+
+
+datatype calc =
+  Cadd int
+  | Csub int
+  | Cmul int
+  | Cdiv int
+  | Creset int
+  | Cskip
+
+(*
+datatype calc_st = CSi int
+*)
+definition calc_sem :: "calc \<Rightarrow> int \<Rightarrow> int" where
+"calc_sem syn st = 
+  (case syn of
+     (Cadd i) \<Rightarrow> st + i
+    |(Csub i) \<Rightarrow> st - i
+    |(Cmul i) \<Rightarrow> st * i
+    |(Cdiv i) \<Rightarrow> divide_int_inst.divide_int st i
+    |(Creset i) \<Rightarrow> i
+    | Cskip \<Rightarrow> st)"
+
+
+
+(* need "liftable" typeclass"? *)
+
+datatype print =
+  Pprint
+  | Preset
+  | Pskip
+
+
+type_synonym state = "int md_triv option md_prio * int list md_triv option"
+
+datatype syn =
+  Sadd int
+  | Ssub int
+  | Smul int
+  | Sdiv int
+  | Sreset int
+  | Sskip
+
+definition print_trans :: "syn \<Rightarrow> print" where
+"print_trans c = 
+  (case c of
+    Sreset _ \<Rightarrow> Preset
+    | Sskip \<Rightarrow> Pskip
+    | _ \<Rightarrow> Pprint)"
+
+definition calc_trans :: "syn \<Rightarrow> calc" where
+"calc_trans c =
+  (case c of
+    Sadd i \<Rightarrow> (Cadd i)
+    | Ssub i \<Rightarrow> (Csub i)
+    | Smul i \<Rightarrow> (Cmul i)
+    | Sdiv i \<Rightarrow> (Cdiv i)
+    | Sreset i \<Rightarrow> (Creset i)
+    | Sskip \<Rightarrow> Cskip)"
+    
+
+type_synonym print_st = "(int * int list)"
+definition print_sem :: "print \<Rightarrow> print_st \<Rightarrow> print_st" where
+"print_sem syn st =
+  (case st of
+    (sti, stl) \<Rightarrow>
+      (case syn of
+         Pprint \<Rightarrow> (sti, stl @ [sti])
+         | Preset \<Rightarrow> (sti, [])))"
+
+definition print_sem_l :: "syn \<Rightarrow> state \<Rightarrow> state" where
+  "print_sem_l = 
+    l_map2' (print_trans)
+            (prod_l ((prio_l_zero (option_l (triv_l (id_l)))))
+                    ((option_l (triv_l (id_l))))) print_sem"
+
+(*
+definition calc_sem_l :: "syn \<Rightarrow> state \<Rightarrow> state" where
+"calc_sem_l =
+  l_map2' calc_trans
+    (fst_l (prio_l_inc (option_l (triv_l (id_l))))) calc_sem"
+*)
+
+definition calc_sem_l :: "syn \<Rightarrow> state \<Rightarrow> state" where
+"calc_sem_l =
+  l_map2' calc_trans
+    (fst_l (prio_l_inc (option_l (triv_l (id_l))))) calc_sem"
+
+definition print_calc_lc :: "(syn, state) langcomp" where
+"print_calc_lc =
+  \<lparr> Sem1 = calc_sem_l
+  , Sem2 = print_sem_l \<rparr>"
+
+value "pcomp print_calc_lc (Smul 9) (mdp 0 (Some (mdt 1)), Some (mdt []))"
+value "pcomp' print_calc_lc (Smul 2) (mdp 0 (Some (mdt 1)), Some (mdt []))"
+
+lemma ex_lc_valid :
+  "lc_valid print_calc_lc" 
+  apply(rule lc_valid_lift)
+   apply(simp add: print_calc_lc_def calc_sem_l_def print_sem_l_def)
+  apply(rule sup_l_comm)
+  apply(rule sup_l_prod_fst)
+  apply(rule sup_l_inc_zero)
+  done
+  
+
+
+end
